coq/exec/MemInv.v
@@ -1,0 +1,66 @@
+Require Import syntax.
+Require Import alist.
+Require Import FMapWeakList.
+
+Require Import Coqlib.
+Require Import infrastructure.
+Require Import Metatheory.
+Require Import vellvm.
+Import Opsem.
+
+Require Import Exprs.
+Require Import Hints.
+Require Import GenericValues.
+
+Set Implicit Arguments.
+
+(* TODO: global, le_public *)
+
+Module Unary.
+  Structure t := mk {
+    global: mblock;
+    private: list mblock;
+    private_parent: list mblock;
+  }.
+
+  Inductive sem (conf:Config) (shared:mblock -> Prop) (inv:t): Prop :=
+  | sem_intro
+      (GLOBAL: True)
+      (PRIVATE: forall b (IN: In b inv.(private)), ~ shared b)
+      (PRIVATE_PARENT: forall b (IN: In b inv.(private_parent)), ~ shared b)
+  .
+
+  Inductive le (lhs rhs:t): Prop :=
+  | le_intro
+      (GLOBAL: lhs.(global) = rhs.(global))
+      (PARENT: lhs.(private_parent) = rhs.(private_parent))
+  .
+End Unary.
+
+Module Relational.
+  Structure t := mk {
+    src: Unary.t;
+    tgt: Unary.t;
+    inject: meminj;
+  }.
+
+  Definition shared_src (inv:t) (b:mblock): Prop :=
+    inv.(inject) b <> None.
+
+  Definition shared_tgt (inv:t) (b:mblock): Prop :=
+    exists b_src offset, inv.(inject) b_src = Some (b, offset).
+
+  Inductive sem (conf_src conf_tgt:Config) (mem_src mem_tgt:mem) (inv:t): Prop :=
+  | sem_intro
+      (SRC: Unary.sem conf_src (shared_src inv) inv.(src))
+      (TGT: Unary.sem conf_tgt (shared_tgt inv) inv.(tgt))
+      (INJECT: Mem.inject inv.(inject) mem_src mem_tgt)
+  .
+
+  Inductive le (lhs rhs:t): Prop :=
+  | le_intro
+      (SRC: Unary.le lhs.(src) rhs.(src))
+      (TGT: Unary.le lhs.(tgt) rhs.(tgt))
+      (INJECT: inject_incr lhs.(inject) rhs.(inject))
+  .
+End Relational.
